packages/forge-core/src/rules/hs/RulesTest.hs
@@ -1,55 +1,77 @@
-{-# LANGUAGE NoImplicitPrelude #-}
-
 -- | Property tests for rules
-module RulesTest where
+module Main where
 
-import Prelude hiding (undefined, error, head, tail, fromJust)
-import Rules.Core (TaskCompletion(..), verifyCompletion)
+import Prelude hiding (undefined, error, head, tail)
+import qualified Rules.Core as Core
 import Rules.TypeSafety (explicitDefault, explicitConditional)
-import Rules.Verification (VerificationChecklist(..), verifyChecklist)
+import qualified Rules.Verification as V
 import Test.QuickCheck
 
+-- | Arbitrary instance for TaskCompletion
+instance Arbitrary Core.TaskCompletion where
+  arbitrary = Core.TaskCompletion
+    <$> arbitrary
+    <*> arbitrary
+    <*> arbitrary
+    <*> arbitrary
+    <*> arbitrary
+    <*> arbitrary
+
+-- | Arbitrary instance for VerificationChecklist
+instance Arbitrary V.VerificationChecklist where
+  arbitrary = V.VerificationChecklist
+    <$> arbitrary
+    <*> arbitrary
+    <*> arbitrary
+    <*> arbitrary
+    <*> arbitrary
+    <*> arbitrary
+    <*> arbitrary
+    <*> arbitrary
+    <*> arbitrary
+    <*> arbitrary
+
 -- | Property: Task completion requires all verifications
-prop_taskCompletionRequiresAll :: TaskCompletion -> Property
+prop_taskCompletionRequiresAll :: Core.TaskCompletion -> Property
 prop_taskCompletionRequiresAll tc =
-  verifyCompletion tc ==>
-    codeCompiles tc &&
-    typeChecks tc &&
-    testsPass tc &&
-    documentationUpdated tc &&
-    workspaceClean tc &&
-    noTechnicalDebt tc
+  Core.verifyCompletion tc ==>
+    Core.codeCompiles tc &&
+    Core.typeChecks tc &&
+    Core.testsPass tc &&
+    Core.documentationUpdated tc &&
+    Core.workspaceClean tc &&
+    Core.noTechnicalDebt tc
 
 -- | Property: explicitDefault preserves type safety
 prop_explicitDefaultTypeSafe :: Maybe Int -> Int -> Property
-prop_explicitDefaultTypeSafe opt default =
-  let result = explicitDefault opt default
+prop_explicitDefaultTypeSafe opt def =
+  let result = explicitDefault opt def
   in case opt of
-    Nothing -> result === default
+    Nothing -> result === def
     Just value -> result === value
 
 -- | Property: explicitConditional is deterministic
 prop_explicitConditionalDeterministic :: Bool -> Int -> Int -> Property
-prop_explicitConditionalDeterministic cond value default =
-  let result = explicitConditional cond value default
+prop_explicitConditionalDeterministic cond value def =
+  let result = explicitConditional cond value def
   in if cond
      then result === value
-     else result === default
+     else result === def
 
 -- | Property: Verification checklist requires all checks
-prop_verificationRequiresAll :: VerificationChecklist -> Property
+prop_verificationRequiresAll :: V.VerificationChecklist -> Property
 prop_verificationRequiresAll vc =
-  verifyChecklist vc ==>
-    filesReadCompletely vc &&
-    dependencyGraphTraced vc &&
-    allInstancesFixed vc &&
-    noBannedConstructs vc &&
-    typesExplicit vc &&
-    typeChecksPass vc &&
-    testsPass vc &&
-    proofsCheck vc &&
-    documentationUpdated vc &&
-    workspaceClean vc
+  V.verifyChecklist vc ==>
+    V.filesReadCompletely vc &&
+    V.dependencyGraphTraced vc &&
+    V.allInstancesFixed vc &&
+    V.noBannedConstructs vc &&
+    V.typesExplicit vc &&
+    V.typeChecksPass vc &&
+    V.testsPass vc &&
+    V.proofsCheck vc &&
+    V.documentationUpdated vc &&
+    V.workspaceClean vc
 
 -- | Run all tests
 main :: IO ()
